theories/approxis/examples/security_aux.v
@@ -4,6 +4,7 @@ From clutch.approxis Require Import approxis map list.
 Set Default Proof Using "Type*".
 
 Definition TOption (T : type) : type := (TUnit + T)%ty.
+Definition lrel_option {Σ} (A : lrel Σ) := (() + A)%lrel.
 
 Definition opt_mult : val :=
   λ:"opt",
@@ -19,6 +20,32 @@ Definition opt_mult : val :=
 Fact opt_mult_typed (A : type) : (⊢ᵥ opt_mult : (TOption (TOption A) → TOption A)%ty).
 Proof.
   rewrite /opt_mult. tychk.
+Qed.
+
+Definition opt_mult_poly : val :=
+  Λ: λ:"opt",
+    match: "opt" with
+    | NONE => NONE
+    | SOME "vopt" =>
+        match: "vopt" with
+        | NONE => NONE
+        | SOME "v" => SOME "v"
+        end
+    end.
+
+Fact opt_mult_poly_typed : (⊢ᵥ opt_mult_poly : ∀: (TOption (TOption #0) → TOption #0)%ty).
+Proof.
+  rewrite /opt_mult_poly. constructor. tychk.
+Qed.
+
+Fact opt_mult_poly_sem_typed `{!approxisRGS Σ} :
+  ⊢ (∀ A : lrel Σ, lrel_option (lrel_option A) → lrel_option A)%lrel
+      opt_mult_poly opt_mult_poly.
+Proof.
+  replace (∀ A : lrel Σ, lrel_option (lrel_option A) → lrel_option A)%lrel
+    with (interp (∀: TOption (TOption #0) → TOption #0) []) by easy.
+  iApply fundamental_val.
+  rewrite /opt_mult_poly. constructor. tychk.
 Qed.
 
 
